@prefix rdfs: <http://www.w3.org/2000/01/rdf-schema> .
@prefix owl: <http://www.w3.org/2002/07/owl> .
@prefix dct: <http://purl.org/dc/terms/> .
@prefix skos: <http://www.w3.org/2004/02/skos/core> .
@prefix rdf: <http://www.w3.org/1999/02/22-rdf-syntax-ns> .
@prefix xsd: <http://www.w3.org/2001/XMLSchema> .
@prefix foaf: <http://xmlns.com/foaf/0.1/> .
@prefix vs: <http://www.w3.org/2003/06/sw-vocab-status/ns#> .

@prefix ccg: <https://example.org> .

@prefix mtg: <https://example.org/MagicTheGathering/> .

mtg:MagicTheGathering a ccg:CardGame ;
    skos:prefLabel "Magic: The Gathering"@en ;
    rdfs:label "Magic: The Gathering"@en .

mtg:Deck a ccg:CardPool ;
    skos:prefLabel "Deck"@en ;
    rdfs:label "Deck"@en ;
    dct:description "the deck of cards that a player draws from"@en ;
    owl:equivalentClass [
        a owl:Restriction ;
        owl:onProperty ccg:hasCardCount ;
        owl:allValuesFrom [
            a owl:Class ;
            owl:unionOf (
            [
                a owl:Restriction ;
                owl:onProperty ccg:hasCardCount ;
                owl:someValuesFrom ccg:CardSet ;
                owl:maxCardinality 4
             ]
             [
                 a owl:Restriction ;
                 owl:onProperty ccg:hasCardCount ;
                 owl:someValuesFrom ccg:Deck ;
                 owl:maxCardinality 60
              ]
              [
                  a owl:Restriction ;
                  owl:onProperty ccg:hasCardCount ;
                  owl:someValuesFrom ccg:Deck ;
                  owl:minCardinality 40
              ]
              )
        ]
] .

mtg:Mana a ccg:Resource ;
    skos:prefLabel "Mana"@en ;
    rdfs:label "Mana"@en ;
    dct:description "Mana is required for deploying cards and activating abilities. It can come in five six variations."@en ;

mtg:LandCard a ccg:Card ;
    skos:prefLabel "Land Card"@en ;
    rdfs:label "Lan Card"@en ;
    dct:description "Land cards are used to produce Mana. Some lands have other special effects."@en ;
    ccg:hasEffect [
        a ccg:Effect .
    ] .

# CreatureCard
ccg:CreatureCard a owl:Class ;
    rdfs:subClassOf ccg:PermanentCard ;
    rdfs:label "Creature Card"@en ;
    rdfs:comment "Represents cards that depict creatures, characters, or entities within the game."@en ;
    ccg:isType mtg:Permanent .

# SpellCard
ccg:SpellCard a owl:Class ;
    rdfs:subClassOf ccg:Card ;
    rdfs:label "Spell Card"@en ;
    rdfs:comment "Represents cards that cast spells, perform actions, or have immediate effects."@en .

# ArtifactCard
ccg:ArtifactCard a owl:Class ;
    rdfs:subClassOf ccg:PermanentCard ;
    rdfs:label "Artifact Card"@en ;
    rdfs:comment "Represents cards that depict magical items, equipment, or artifacts."@en .

# EnchantmentCard
ccg:EnchantmentCard a owl:PermanentClass ;
    rdfs:subClassOf ccg:Card ;
    rdfs:label "Enchantment Card"@en ;
    rdfs:comment "Represents cards that provide continuous effects or modify game rules."@en .

# LandCard
ccg:LandCard a owl:Class ;
    rdfs:subClassOf ccg:PermanentCard ;
    rdfs:label "Land Card"@en ;
    rdfs:comment "Represents cards that provide resources or have special abilities related to the game environment."@en .
