@prefix rdfs: <http://www.w3.org/2000/01/rdf-schema> .
@prefix owl: <http://www.w3.org/2002/07/owl> .
@prefix dct: <http://purl.org/dc/terms/> .
@prefix skos: <http://www.w3.org/2004/02/skos/core> .
@prefix rdf: <http://www.w3.org/1999/02/22-rdf-syntax-ns> .
@prefix xsd: <http://www.w3.org/2001/XMLSchema> .
@prefix foaf: <http://xmlns.com/foaf/0.1/> .
@prefix vs: <http://www.w3.org/2003/06/sw-vocab-status/ns#> .

@prefix ccg: <https://example.org> .

@prefix mtg: <https://example.org/MagicTheGathering/> .

mtg:MagicTheGathering a ccg:CardGame ;
    skos:prefLabel "Magic: The Gathering"@en ;
    rdfs:label "Magic: The Gathering"@en .

mtg:Deck a ccg:CardPool ;
    skos:prefLabel "Deck"@en ;
    rdfs:label "Deck"@en ;
    dct:description "the deck of cards that a player draws from"@en ;
    owl:equivalentClass [
        a owl:Restriction ;
        owl:onProperty ccg:hasCardCount ;
        owl:allValuesFrom [
            a owl:Class ;
            owl:unionOf (
            [
                a owl:Restriction ;
                owl:onProperty ccg:hasCardCount ;
                owl:someValuesFrom ccg:CardSet ;
                owl:maxCardinality 4
             ]
             [
                 a owl:Restriction ;
                 owl:onProperty ccg:hasCardCount ;
                 owl:someValuesFrom ccg:Deck ;
                 owl:maxCardinality 60
              ]
              [
                  a owl:Restriction ;
                  owl:onProperty ccg:hasCardCount ;
                  owl:someValuesFrom ccg:Deck ;
                  owl:minCardinality 40
              ]
              )
        ]
] .

mtg:ToughnessStat a ccg:CardStat ;
    skos:prefLabel "Toughness"@en ;
    rdfs:label "Toughness"@en .

mtg:PowerStat a ccg:CardStat ;
    skos:prefLabel "Power"@en !
    rdfs:label "Power"@en .

mtg:Battlefield rdf:type ccg:PlayArea ;
    ccg:hasPlayZone mtg:Library, mtg:Graveyard .

mtg:Library a ccg:HiddenZone ;
    ccg:hasCardPool ccg:Deck .

mtg:Graveyard a ccg:Public zone ;
    ccg:hasCardPool ccg:DiscardPile .

mtg:TapAction a owl:Class ;
    rdfs:subClassOf ccg:ActivateAction ;
    skos:prefLabel "Tap"@en ;
    rdfs:label "Tap"@en ;
    dct:description "To Tap your card, you turn it sideways. This is how you activate a card in Magic."@en .

mtg:Mana a ccg:Resource ;
    skos:prefLabel "Mana"@en ;
    rdfs:label "Mana"@en ;
    dct:description "Mana is required for deploying cards and activating abilities. It can come in five six variations."@en ;

mtg:GreenMana a owl:Class ;
    rdfs:subClassOf mtg:Mana ;
    skos:prefLabel "Green Mana"@en ;
    rdfs:label "Green Mana"@en ;
    dct:description "Green Mana is generally produced by Forest Cards"@en .

mtg:WhiteMana a owl:Class ;
    rdfs:subClassOf mtg:Mana ;
    skos:prefLabel "White Mana"@en ;
    rdfs:label "White Mana"@en ;
    dct:description "White Mana is generally produced by Plains Cards"@en .

mtg:BlackMana a owl:Class ;
    rdfs:subClassOf mtg:Mana ;
    skos:prefLabel "Black Mana"@en ;
    rdfs:label "Black Mana"@en ;
    dct:description "Black Mana is generally produced by Swamp Cards"@en .

mtg:BlueMana a owl:Class ;
    rdfs:subClassOf mtg:Mana ;
    skos:prefLabel "Blue Mana"@en ;
    rdfs:label "Blue Mana"@en ;
    dct:description "Blue Mana is generally produced by FlIsland Cards"@en .

mtg:RedMana a owl:Class ;
    rdfs:subClassOf mtg:Mana ;
    skos:prefLabel "Red Mana"@en ;
    rdfs:label "Red Mana"@en ;
    dct:description "Red Mana is generally produced by Mountain Cards"@en .

mtg:LandCard a ccg:PermanentCard ;
    skos:prefLabel "Land Card"@en ;
    rdfs:label "Lan Card"@en ;
    dct:description "Land cards are used to produce Mana. Some lands have other special effects."@en .

ccg:Forest a ccg:LandCard ;
    skos:prefLabel "Forest"@en ;
    rdfs:label "Forest"@en ;
    dct:description "Generates a Green Mana when tapped."@en ;
    ccg:hasEffect [
        a ccg:Effect ;
        ccg:hasTrigger mtg:TapAction ;
        ccg:hasAction [
            a ccg:ResourceAction ;
            ccg:hasSideEffect [
                a mtg:ManaPool ;
                ccg:hasResource mtg:GreenMana ;
                ccg:hasResourceCount 1;
            ] ;
        ] ;
    ] .

ccg:Plains a ccg:LandCard ;
    skos:prefLabel "Plains"@en ;
    rdfs:label "Plains"@en ;
    dct:description "Generates a White Mana when tapped."@en ;
    ccg:hasEffect [
        a ccg:Effect ;
        ccg:hasTrigger mtg:TapAction ;
        ccg:hasAction [
            a ccg:ResourceAction ;
            ccg:hasSideEffect [
                a mtg:ManaPool ;
                ccg:hasResource mtg:WhiteMana ;
                ccg:hasResourceCount 1;
            ] ;
        ] ;
    ] .

ccg:Island a ccg:LandCard ;
    skos:prefLabel "Island"@en ;
    rdfs:label "Island"@en ;
    dct:description "Generates a Blue Mana when tapped."@en ;
    ccg:hasEffect [
        a ccg:Effect ;
        ccg:hasTrigger mtg:TapAction ;
        ccg:hasAction [
            a ccg:ResourceAction ;
            ccg:hasSideEffect [
                a mtg:ManaPool ;
                ccg:hasResource mtg:BlueMana ;
                ccg:hasResourceCount 1;
            ] ;
        ] ;
    ] .

ccg:Swamp a ccg:LandCard ;
    skos:prefLabel "Swamp"@en ;
    rdfs:label "Swamp"@en ;
    dct:description "Generates a Black Mana when tapped."@en ;
    ccg:hasEffect [
        a ccg:Effect ;
        ccg:hasTrigger mtg:TapAction ;
        ccg:hasAction [
            a ccg:ResourceAction ;
            ccg:hasSideEffect [
                a mtg:ManaPool ;
                ccg:hasResource mtg:BlackMana ;
                ccg:hasResourceCount 1;
            ] ;
        ] ;
    ] .

ccg:Mountain a ccg:LandCard ;
    skos:prefLabel "Mountain"@en ;
    rdfs:label "Mountain"@en ;
    dct:description "Generates a Red Mana when tapped."@en ;
    ccg:hasEffect [
        a ccg:Effect ;
        ccg:hasTrigger mtg:TapAction ;
        ccg:hasAction [
            a ccg:ResourceAction ;
            ccg:hasSideEffect [
                a mtg:ManaPool ;
                ccg:hasResource mtg:RedMana ;
                ccg:hasResourceCount 1;
            ] ;
        ] ;
    ] .

ccg:LibraryOfLeng a ccg:ArtifactCard ;
    skos:prefLabel "Library of Leng"@en ;
    rdfs:label "Library of Leng"@en ;
    ccg:hasRuleText "You have no maximum hand size. If an effect causes you to discard a card, discard it, but you may put it on top of your library instead of into your graveyard."@en ;
    ccg:hasEffect [
        a ccg:Effect ;
        ccg:hasTrigger mtg:DiscardAction ;
        ccg:hasAction [
            a ccg:ChoiceAction ;
            ccg:hasOption [
                a ccg:DiscardOption ;
                ccg:hasDestination mtg:Graveyard ;
            ] ;
            ccg:hasOption [
                a ccg:DiscardOption ;
                ccg:hasDestination mtg:LibraryTop ;
            ] ;
        ] ;
    ccg:hasEffect [
        a ccg:Effect ;
        ccg:hasCondition mtg:NoMaximumHandSizeCondition ;
    ] ;
] .

ccg:LightningBolt a ccg:InstantCard ;
    skos:prefLabel "Lightning Bolt"@en ;
    rdfs:label "Lightning Bolt"@en ;
    ccg:hasRuleText "Lightning Bolt deals 3 damage to any target."@en ;
    ccg:hasEffect [
        a ccg:Effect ;
        ccg:hasTrigger mtg:CastAction ;
        ccg:hasAction [
            a ccg:DamageAction ;
            ccg:hasAmount 3 ;
            ccg:hasTarget mtg:AnyTarget ;
        ] ;
    ] .

ccg:StripMine a ccg:LandCard ;
    skos:prefLabel "Strip Mine"@en ;
    rdfs:label "Strip Mine"@en ;
    ccg:hasRuleText "Adds 1 colorless mana to your mana pool or sacrifices to destroy target land."@en ;
    ccg:hasEffect [
        a ccg:Effect ;
        ccg:hasTrigger mtg:TapAction ;
        ccg:hasAction [
            a ccg:ResourceAction ;
            ccg:hasSideEffect [
                a mtg:ManaPool ;
                ccg:hasResource mtg:ColorlessMana ;
                ccg:hasResourceCount 1 ;
            ] ;
        ] ;
    ],
    [
        a ccg:Effect ;
        ccg:hasTrigger mtg:SacrificeAction ;
        ccg:hasAction [
            a ccg:DestroyAction ;
            ccg:hasTarget mtg:LandCard ;
        ] ;
    ] .

ccg:LlanowarElves a ccg:CreatureCard ;
    skos:prefLabel "Llanowar Elves"@en ;
    rdfs:label "Llanowar Elves"@en ;
    dct:description "One of the most well-known creatures, Llanowar Elves have been used by generations of players for mana acceleration."@en ;
    ccg:hasRuleText "{T}: Add {G}."@en ;
    ccg:hasManaCost [
        a ccg:ManaCost ;
        ccg:requiresMana mtg:GreenMana ;
        ccg:requiresManaCount 1 ;
    ] ;
    ccg:hasStat [
        a mtg:ToughnessStat ;
        ccg:hasCurrentValue 1 .
    ] ;
    ccg:hasStat [
        a mtg:PowerStat ;
        ccg:hasCurrentValue 1 .
    ] ;
    ccg:hasEffect [
        a ccg:Effect ;
        ccg:hasTrigger mtg:TapAction ;
        ccg:hasAction [
            a ccg:ResourceAction ;
            ccg:hasSideEffect [
                a mtg:ManaPool ;
                ccg:hasResource mtg:GreenMana ;
                ccg:hasResourceCount 1 ;
            ] ;
        ] ;
    ] .

ccg:SolRing a ccg:ArtifactCard ;
    skos:prefLabel "Sol Ring"@en ;
    rdfs:label "Sol Ring"@en ;
    dct:description "Provides an abundant source of mana by tapping into the core of a distant star."@en ;
    ccg:hasRuleText "{T}: Add {C}{C}."@en ;
    ccg:hasManaCost [
        a ccg:ManaCost ;
        ccg:requiresMana mtg:ColorlessMana ;
        ccg:requiresManaCount 1 ;
    ] ;
    ccg:hasEffect [
        a ccg:Effect ;
        ccg:hasTrigger mtg:TapAction ;
        ccg:hasAction [
            a ccg:ResourceAction ;
            ccg:hasSideEffect [
                a mtg:ManaPool ;
                ccg:hasResource mtg:ColorlessMana ;
                ccg:hasResourceCount 2 ;
            ] ;
        ] ;
    ] .

ccg:GiantGrowth a ccg:InstantCard ;
    skos:prefLabel "Giant Growth"@en ;
    rdfs:label "Giant Growth"@en ;
    ccg:hasRuleText "Target creature gets +3/+3 until end of turn."@en ;
    ccg:hasEffect [
        a ccg:Effect ;
        ccg:hasTrigger mtg:CastAction ;
        ccg:hasTarget mtg:CreatureCard ;
        ccg:hasAction [
            a ccg:ModifyPTAction ;
            ccg:hasAmount 3 ;
            ccg:hasDuration mtg:EndOfTurn ;
        ] ;
    ] .


# CreatureCard
ccg:CreatureCard a owl:Class ;
    rdfs:subClassOf ccg:PermanentCard ;
    rdfs:label "Creature Card"@en ;
    rdfs:comment "Represents cards that depict creatures, characters, or entities within the game."@en ;
    ccg:isType mtg:Permanent .

# SpellCard
ccg:SpellCard a owl:Class ;
    rdfs:subClassOf ccg:Card ;
    rdfs:label "Spell Card"@en ;
    rdfs:comment "Represents cards that cast spells, perform actions, or have immediate effects."@en .

ccg:InstantCard a owl:Class ;
    rdfs:subClassOf ccg:SpellCard ;
    rdfs:label "Instant"@en ;
    rdfs:comment "Represents cards that take effect instantly."@en .

# ArtifactCard
ccg:ArtifactCard a owl:Class ;
    rdfs:subClassOf ccg:PermanentCard ;
    rdfs:label "Artifact Card"@en ;
    rdfs:comment "Represents cards that depict magical items, equipment, or artifacts."@en .

# EnchantmentCard
ccg:EnchantmentCard a ccg:PermanentCard ;
    rdfs:subClassOf ccg:Card ;
    rdfs:label "Enchantment Card"@en ;
    rdfs:comment "Represents cards that provide continuous effects or modify game rules."@en .

mtg:Comprehensive rules a ccg:RuleBook ;
    dct:title "Magic: The Gathering Comprehensive Rules"@en ;
    ccg:hasRuleSection mtg:GameConcepts .

mtg:GameConceptsRuleSection a ccg:RuleSection ;
    dct:title "Game Concepts"@en ;
    ccg:hasSubSection ccg:GeneralRulesSection ;

mtg:GeneralRulesSection a ccg:RulesSection ;
    dct:title "1. General"@en .

mtg:Rule100%2e1 a ccg:Rule ;
    ccg:isDefinedIn mtg:GeneralRulesSection ;
    dct:description "100.1. These Magic rules apply to any Magic game with two or more players, including two-player games and multiplayer games."@en .

mtg:Rule100%2e1a a ccg:Rule ;
    ccg:isDefinedIn mtg:GeneralRulesSection ;
    skos:related mtg:Player ;
    dct:description "100.1a A two-player game is a game that begins with only two players."@en .

mtg:Rule100%2e1b a ccg:Rule ;
    ccg:isDefinedIn mtg:GeneralRulesSection ;
    rdfs:seeAlso mtg:MultiplayerRulesSection ;
    skos:related mtg:Player ;
    dct:description "100.1b A multiplayer game is a game that begins with more than two players. See section 8, &quot;Multiplayer Rules.&quot;"@en .

mtg:Rule100%2e2 a ccg:Rule ;
    ccg:isDefinedIn mtg:GeneralRulesSection ;
    skos:related mtg:Player ;
    skos:related mtg:Deck ;
    dct:description "100.2. To play, each player needs their own deck of traditional Magic cards, small items to represent any tokens and counters, and some way to clearly track life totals."@en .

mtg:Rule100%2e2a a ccg:Rule ;
    ccg:isDefinedIn mtg:GeneralRulesSection ;
    rdfs:seeAlso mtg:Rule201%2e3 ;
    skos:related mtg:Player ;
    skos:related mtg:Deck ;
    dct:description "100.2a In constructed play (a way of playing in which each player creates their own deck ahead of time), each deck has a minimum deck size of 60 cards. A constructed deck may contain any number of basic land cards and no more than four of any card with a particular English name other than basic land cards. For the purposes of deck construction, cards with interchangeable names have the same English name (see rule 201.3)."@en .

mtg:Rule100%2e2b a ccg:Rule ;
    ccg:isDefinedIn mtg:GeneralRulesSection ;
    skos:related mtg:Player ;
    skos:related mtg:Deck ;
    dct:description "100.2b In limited play (a way of playing in which each player gets the same quantity of unopened Magic product such as booster packs and creates their own deck using only this product and basic land cards), each deck has a minimum deck size of 40 cards. A limited deck may contain as many duplicates of a card as are included with the product."@en .

mtg:Rule100%2e2c a ccg:Rule ;
    ccg:isDefinedIn mtg:GeneralRulesSection ;
    rdfs:seeAlso mtg:Rule903 ;
    skos:related mtg:Deck ;
    dct:description "100.2c Commander decks are subject to additional deckbuilding restrictions and requirements. See rule 903, &quot;Commander,&quot; for details."@en .

mtg:Rule100%2e2d a ccg:Rule ;
    ccg:isDefinedIn mtg:GeneralRulesSection ;
    rdfs:seeAlso mtg:Rule108%2e2a ;
    rdfs:seeAlso mtg:Rule717 ;
    rdfs:seeAlso mtg:Rule901 ;
    rdfs:seeAlso mtg:Rule904 ;
    skos:related mtg:Player ;
    skos:related mtg:Deck ;
    dct:description "100.2d Some formats and casual play variants allow players to use a supplementary deck of nontraditional Magic cards (see rule 108.2a). These supplementary decks have their own deck construction rules. See rule 717, &quot;Attraction Cards;&quot; rule 901, &quot;Planechase;&quot; and rule 904, &quot;Archenemy.&quot;"@en .

mtg:Rule100%2e3 a ccg:Rule ;
    ccg:isDefinedIn mtg:GeneralRulesSection ;
    skos:related mtg:Card ;
    dct:description "100.3. Some cards require coins or traditional dice. Some casual variants require additional items, such as specially designated cards, nontraditional Magic cards, and specialized dice."@en .

mtg:Rule100%2e4 a ccg:Rule ;
    ccg:isDefinedIn mtg:GeneralRulesSection ;
    skos:related mtg:Card ;
    skos:related mtg:Player ;
    skos:related mtg:Sideboard ;
    skos:related mtg:Deck ;
    dct:description "100.4. Each player may also have a sideboard, which is a group of additional cards the player may use to modify their deck between games of a match."@en .

mtg:Rule100%2e4a a ccg:Rule ;
    ccg:isDefinedIn mtg:GeneralRulesSection ;
    rdfs:seeAlso mtg:Rule100%2e2a ;
    skos:related mtg:Sideboard ;
    skos:related mtg:Deck ;
    dct:description "100.4a In constructed play, a sideboard may contain no more than fifteen cards. The four-card limit (see rule 100.2a) applies to the combined deck and sideboard."@en .

mtg:Rule100%2e4b a ccg:Rule ;
    ccg:isDefinedIn mtg:GeneralRulesSection ;
    skos:related mtg:Player ;
    skos:related mtg:Sideboard ;
    skos:related mtg:Deck ;
    dct:description "100.4b In limited play involving individual players, all cards in a player’s card pool not included in their deck are in that player’s sideboard."@en .

mtg:Rule100%2e4c a ccg:Rule ;
    ccg:isDefinedIn mtg:GeneralRulesSection ;
    skos:related mtg:Player ;
    skos:related mtg:Sideboard ;
    skos:related mtg:Deck ;
    dct:description "100.4c In limited play involving the Two-Headed Giant multiplayer variant, all cards in a team’s card pool but not in either player’s deck are in that team’s sideboard.
"@en .

mtg:Rule100%2e4d a ccg:Rule ;
    ccg:isDefinedIn mtg:GeneralRulesSection ;
    skos:related mtg:Player ;
    skos:related mtg:Sideboard ;
    skos:related mtg:Card ;
    dct:description "100.4d In limited play involving other multiplayer team variants, each card in a team’s card pool but not in any player’s deck is assigned to the sideboard of one of those players. Each player has their own sideboard; cards may not be transferred between players."@en .

mtg:Rule100%2e5 a ccg:Rule ;
    ccg:isDefinedIn mtg:GeneralRulesSection ;
    skos:related mtg:Card ;
    skos:related mtg:Deck ;
    dct:description "100.5. If a deck must contain at least a certain number of cards, that number is referred to as a minimum deck size. There is no maximum deck size for non-Commander decks."@en .