@prefix rdfs: <http://www.w3.org/2000/01/rdf-schema> .
@prefix owl: <http://www.w3.org/2002/07/owl> .
@prefix dct: <http://purl.org/dc/terms/> .
@prefix skos: <http://www.w3.org/2004/02/skos/core> .
@prefix rdf: <http://www.w3.org/1999/02/22-rdf-syntax-ns> .
@prefix xsd: <http://www.w3.org/2001/XMLSchema> .
@prefix foaf: <http://xmlns.com/foaf/0.1/> .
@prefix vs: <http://www.w3.org/2003/06/sw-vocab-status/ns#> .

@prefix ccg: <https://example.org>

ccg: rdf:type owl:Ontology ;
    skos:prefLabel "Collectible Card Game Ontology" ;
    dct:description "This Ontology is intended to provide a comprehensive way of representing CCG's in a semantic way." ;
    rdfs:comment "This Ontology exists to encode the rules and concepts of Collectible Card Games into a machine readable format." ;
    owl:versionInfo "1.0" ;
    dct:creator "Brent Ritchie" ;
    dct:title "Collectible Card Game Ontology" ;
    rdfs:label "CCG Ontology" ;
    dct:created "2024-05-12" ;
    dct:issued "2024-05-12" ;
    foaf:mbox "ritchie.brent@gmail.com" ;
    dct:language "en" ;
    dct:audience "Intended for anyone interested in the semantic representation of CCG's." ;
    skos:scopeNote "Intended to be used for understanding digital and print CCG's" ;
    vs:term_status "stable" ;
    owl:imports <http://www.w3.org/TR/skos-reference/skos-owl1-dl.rdf> .

# Classes

ccg:CardGame a owl:Class ;
    skos:prefLabel "Card Game"@en ;
    rdfs:label "Card Game"@en ;
    dct:description "Represents a card game that can be played."@en .

ccg:CardSet a owl:Class ;
    skos:prefLabel "Card Set"@en ;
    rdfs:label "Card Set"@en ;
    dct:description "Represents a card set release for a game."@en .

ccg:Card a owl:Class ;
    skos:prefLabel "Card"@en ;
    rdfs:label "Card"@en ;
    dct:Description "The most basic part of a CCG is the Card. These can take many shapes and sizes."@en .

ccg:CardType a owl:Class ;
    skos:prefLabel "Card Type"@en ;
    rdfs:label "Card Type"@en ;
    dct:description "A specific type of card that is distinct from other types in the game."@en ;
    skos:example "Land, Energy, Artifacts, Spells, Tokens."@en .

ccg:Effect a owl:Class .

ccg:CardPool a owl:Class ;
    skos:prefLabel "Card Pool"@en ;
    rdfs:label "Card Pool"@en ;
    dct:description "Any collection of cards that is used as part of the game."@en ;
    skos:example "Deck, hand, discard pile"@en .

ccg:Resource a owl:Ontology ;
    skos:prefLabel "Resource"@en ;
    rdfs:label "Resource"@en ;
    dct:description "Anything that needs to be managed by the player but has no direct physical representation in the game"@en ;
    skos:example "Mana, Player Health"@en .

ccg:CardRarity a owl:Class .

ccg:CardStat a owl:Class .

ccg:PlayZone a owl:Class ;
    skos:prefLabel "Play Zone"@en ;
    rdfs:label "Play Zone"@en ;
    dct:description "Any zone distinct zone that is used as a play area."@en ;
    skos:example "Library, Bench, Active Slot"@en .

# Predicates

ccg:hasSet a owl:ObjectProperty ;
    rdfs:domain ccg:CardGame ;
    rdfs:range ccg:CardSet ;
    skos:prefLabel "has card set"@en ;
    rdfs:label "has card set"@en ;
    dct:description "Relates a card game to its sets of cards. A set is generally a release of cards as a grouping and all having a similar theme."@en .

ccg:hasCard a owl:ObjectProperty ;
    rdfs:domain [
        a owl:Class ;
        owl:unionOf (ccg:CardSet ccg:CardPool) .
    ] ;
    rdfs:range ccg:Card ;
    skos:prefLabel "has card"@en ;
    rdfs:label "has card"@en ;
    dct:description "relates different items that can contain cards like decks, card sets,hands, etc..."@en .

ccg:hasEffect a owl:ObjectProperty ;
    rdfs:domain ccg:Card ;
    rdfs:range ccg:Effect ;
    skos:prefLabel "has effect"@en ;
    rdfs:label "has effect"@en ;
    dct:description "Relates an effect to a card, generally the effect is found in the rule box of the card."@en .

ccg:hasRuleText a owl:objectProperty ;
    rdfs:domain ccg:Card ;
    rdfs:range xsd:string ;
    skos:prefLabel "has rule text"@en ;
    rdfs:label "has rule text"@en ;
    dct:description "Relates the card to the exact rule text that shows up on it."@en .

ccg:isType a owl:ObjectProperty ;
    rdfs:domain ccg:Card ;
    rdfs:range ccg:CardType ;
    skos:prefLabel "is type"@en ;
    rdfs:label "is type"@en ;
    dct:description "Relates a card to a specific game defined type."@en ;

ccg:hasStat a owl:ObjectProperty .

ccg:hasRarity a owl:ObjectProperty .

ccg:hasPool a owl:ObjectProperty .